revise systemF types to delegate to STLC

Lp2lc/Active/F/Def.lean
@@ -5,13 +5,13 @@ import «Lp2lc».Active.STLC
 namespace Lp2lc.Active.F
 
 inductive Typ : Type where
-  | stlc : STLC.Typ
+  | stlc : STLC.Typ -> Typ
   | bvar : Nat -> Typ
   | fvar : Var -> Typ
 deriving DecidableEq, Repr
 
 inductive Trm : Type where
-  | stlc: STLC.Trm
+  | stlc: STLC.Trm -> Trm
   | tabs : Trm -> Trm
   | tapp : Trm -> Typ -> Trm
 deriving DecidableEq, Repr
